sys-init/StaticDerivations_SI.thy
@@ -10,113 +10,115 @@ imports
   Sep_Algebra.Extended_Separation_Algebra
 begin
 
+definition spec_object_size :: "cdl_state \<Rightarrow> cdl_object_id \<Rightarrow> nat" where
+  "spec_object_size spec ptr \<equiv>
+     let obj = the (cdl_objects spec ptr)
+     in obj_bits_cdl (object_type obj) (object_size_bits obj)"
 
-definition "spec_object_size spec ptr =
-  (let obj = (the (cdl_objects spec ptr)) in obj_bits_cdl (object_type obj) (object_size_bits obj))"
+definition next_allocation :: "cdl_state \<Rightarrow> cdl_object_id \<Rightarrow> cdl_object_id \<Rightarrow> cdl_object_id" where
+  "next_allocation spec previous current =
+     alignUp previous (spec_object_size spec current) + 2 ^ (spec_object_size spec current)"
 
-definition "next_allocation spec previous current =
-   alignUp previous (spec_object_size spec current) + 2 ^ (spec_object_size spec current)"
-
+(* FIXME: find better name and move to Lib *)
 fun previous :: "'a \<Rightarrow> 'a list \<Rightarrow> 'a option"  where
   "previous v [] = None" |
   "previous v [x] = None" |
   "previous v (x#y#xs) =  (if y = v then Some x else previous v (y#xs))"
 
-primrec allocate where
-   "allocate base_ptr spec [] = Map.empty" |
-   "allocate ptr spec (x#xs) = [x \<mapsto> ptr] + allocate (next_allocation spec ptr x ) spec xs"
+primrec allocate ::
+  "cdl_object_id \<Rightarrow> cdl_state \<Rightarrow> cdl_object_id list \<Rightarrow> cdl_object_id \<Rightarrow> cdl_object_id option"
+  where
+  "allocate base_ptr spec [] = Map.empty" |
+  "allocate ptr spec (x#xs) = [x \<mapsto> ptr] + allocate (next_allocation spec ptr x) spec xs"
 
 declare allocate.simps[simp del]
 
-definition "mapp g f = (\<lambda>x. map_option (g x) (f x))"
+definition mapp :: "('a \<Rightarrow> 'c \<Rightarrow> 'b) \<Rightarrow> ('a \<Rightarrow> 'c option) \<Rightarrow> 'a \<Rightarrow> 'b option" where
+  "mapp g f \<equiv> \<lambda>x. map_option (g x) (f x)"
 
-definition "aligned_allocations spec base_ptr children =
-      mapp (\<lambda>ptr ptr'. alignUp ptr' (spec_object_size spec ptr)) (allocate base_ptr spec children)"
+definition aligned_allocations ::
+  "cdl_state \<Rightarrow> cdl_object_id \<Rightarrow> cdl_object_id list \<Rightarrow> cdl_object_id \<Rightarrow> cdl_object_id option"
+  where
+  "aligned_allocations spec base_ptr children =
+     mapp (\<lambda>ptr ptr'. alignUp ptr' (spec_object_size spec ptr)) (allocate base_ptr spec children)"
 
-lemma [simp]:
+lemma mapp_plus[simp]:
   "mapp g (x + y) = mapp g x + mapp g y"
-  apply (intro ext iffI; clarsimp simp: mapp_def plus_fun_def plus_option_def split: option.splits)
-  done
+  by (fastforce simp: mapp_def plus_fun_def plus_option_def split: option.splits)
 
-lemma [simp]:
+lemma mapp_singleton[simp]:
   "mapp g ([x \<mapsto> y]) = [x \<mapsto> g x y]"
-  apply (intro ext iffI; clarsimp simp: mapp_def plus_fun_def plus_option_def split: option.splits)
-  done
+  by (fastforce simp: mapp_def plus_fun_def plus_option_def split: option.splits)
 
-lemma aligned_allocations_hd: "aligned_allocations spec ptr (a#list) a =
-  Some (alignUp ptr (spec_object_size spec a))"
+lemma aligned_allocations_hd:
+  "aligned_allocations spec ptr (a#list) a = Some (alignUp ptr (spec_object_size spec a))"
   apply (clarsimp simp: aligned_allocations_def allocate.simps)
   apply (simp add: plus_fun_def plus_option_def)
   done
 
-lemma mapp_app[simp]: "M x \<noteq> None \<Longrightarrow> (mapp f M) x = Some (f x (the (M x)))"
+lemma mapp_app[simp]:
+  "M x \<noteq> None \<Longrightarrow> mapp f M x = Some (f x (the (M x)))"
   by (clarsimp simp: mapp_def)
 
-lemma [simp]: "distinct (x#xs) \<Longrightarrow>
-     ([x \<mapsto> v] + allocate y spec xs) x = Some v"
-  apply (induct xs; clarsimp simp: plus_fun_def plus_option_def)
-  done
+lemma singleton_plus_allocate[simp]:
+  "distinct (x#xs) \<Longrightarrow> ([x \<mapsto> v] + allocate y spec xs) x = Some v"
+  by (induct xs; clarsimp simp: plus_fun_def plus_option_def)
 
-lemma [simp]: "distinct (x#xs) \<Longrightarrow>
-      ([x \<mapsto> v] + mapp g (allocate y spec xs)) x = Some v"
-  apply (induct xs; clarsimp simp: plus_fun_def plus_option_def)
-  done
+lemma singleton_plus_mapp_allocate[simp]:
+  "distinct (x#xs) \<Longrightarrow> ([x \<mapsto> v] + mapp g (allocate y spec xs)) x = Some v"
+  by (induct xs; clarsimp simp: plus_fun_def plus_option_def)
 
-lemma [simp]: "allocate ptr spec (a # list) a = Some ptr"
-  apply (clarsimp simp: allocate.simps)
-  by (simp add: plus_fun_def plus_option_def)
+lemma allocate_hd[simp]:
+  "allocate ptr spec (a # list) a = Some ptr"
+  by (clarsimp simp: allocate.simps plus_fun_def plus_option_def)
 
-lemma not_in_previous: "x \<notin> set list \<Longrightarrow>
-   previous x list = None"
-  apply (induct list arbitrary: x; clarsimp)
-  by (metis list.set_intros(1) not_NilE previous.simps(2) previous.simps(3))
+lemma not_in_previous:
+  "x \<notin> set list \<Longrightarrow> previous x list = None"
+  by (induct list arbitrary: x; clarsimp)
+     (metis list.set_intros(1) not_NilE previous.simps(2) previous.simps(3))
 
-lemma not_in_previous':"x \<notin> set list \<Longrightarrow> Some p = previous x (x # list) \<Longrightarrow> False"
-  apply (induct list arbitrary: x p; clarsimp)
-  by (simp add: not_in_previous)
+lemma not_in_previous':
+  "x \<notin> set list \<Longrightarrow> Some p = previous x (x # list) \<Longrightarrow> False"
+  by (induct list arbitrary: x p; clarsimp)
+     (simp add: not_in_previous)
 
-lemma in_tail_previous: "x \<in> set list \<Longrightarrow> previous x (a # list) \<noteq> None"
+lemma in_tail_previous:
+  "x \<in> set list \<Longrightarrow> previous x (a # list) \<noteq> None"
   by (induct list arbitrary: a; clarsimp)
 
-lemma previous_in_head: "x \<in> set list \<Longrightarrow> the (previous x (a # list)) \<notin> set list
-        \<Longrightarrow> the (previous x (a # list)) = a"
+lemma previous_in_head:
+  "\<lbrakk> x \<in> set list; the (previous x (a # list)) \<notin> set list \<rbrakk> \<Longrightarrow> the (previous x (a # list)) = a"
   by (induct list arbitrary: a; clarsimp)
 
-lemma previous_in_tail: "Some p = previous x (a # list) \<Longrightarrow> x \<in> set list"
+lemma previous_in_tail:
+  "Some p = previous x (a # list) \<Longrightarrow> x \<in> set list"
   by (induct list arbitrary: a; clarsimp split: if_splits)
 
-lemma in_right_map[simp]: "v \<noteq> x \<Longrightarrow> ([x \<mapsto> y] + ys) v = ys v"
- by (clarsimp simp: plus_fun_def plus_option_def)
+lemma in_right_map[simp]:
+  "v \<noteq> x \<Longrightarrow> ([x \<mapsto> y] + ys) v = ys v"
+  by (clarsimp simp: plus_fun_def plus_option_def)
 
-lemma in_list_allocate: "x \<in> set list \<Longrightarrow> \<exists>z. allocate ptr spec (list) x = Some z"
-  apply (induct list arbitrary: ptr x)
-   apply (clarsimp)
-  apply (case_tac "x=a")
-   apply (clarsimp)
-  apply (drule meta_spec)
-  apply (drule_tac x=x in meta_spec)
-  apply (drule meta_mp)
-   apply (clarsimp)
-  apply (clarsimp)
-  apply (rule exI)
-  apply (clarsimp simp: allocate.simps(2))
-  apply (fastforce simp: in_right_map)
+lemma in_list_allocate:
+  "x \<in> set list \<Longrightarrow> \<exists>z. allocate ptr spec (list) x = Some z"
+  apply (induct list arbitrary: ptr x; clarsimp)
+  apply (rename_tac a list ptr x)
+  apply (case_tac "x=a", clarsimp)
+  apply (fastforce simp: allocate.simps(2))
   done
 
-lemma previous_in_list: "previous x list = Some y \<Longrightarrow> y \<in> set list"
-  apply (induct list arbitrary: y)
-   apply clarsimp+
-  apply (metis option.sel previous_in_head previous_in_tail)
-  done
+lemma previous_in_list:
+  "previous x list = Some y \<Longrightarrow> y \<in> set list"
+  by (induct list arbitrary: y; clarsimp)
+     (metis option.sel previous_in_head previous_in_tail)
 
 lemma distinct_previous_const:
   "\<lbrakk>distinct (a#list); previous x list = Some y\<rbrakk> \<Longrightarrow> Some y = previous x (a # list)"
-  apply (induct list arbitrary: x y; clarsimp)
-  apply (metis previous_in_tail)
-  done
+  by (induct list arbitrary: x y; clarsimp)
+     (metis previous_in_tail)
 
-lemma previous_in_allocate: "\<lbrakk>previous x list = Some y; distinct (a#list); x \<in> set list\<rbrakk>
-  \<Longrightarrow> \<exists>z. allocate ptr spec (a # list) y = Some z"
+lemma previous_in_allocate:
+  "\<lbrakk> previous x list = Some y; distinct (a#list); x \<in> set list \<rbrakk> \<Longrightarrow>
+   \<exists>z. allocate ptr spec (a # list) y = Some z"
   apply (drule (1) distinct_previous_const[rotated])
   apply (drule sym)
   apply (frule previous_in_list)
@@ -124,11 +126,11 @@ lemma previous_in_allocate: "\<lbrakk>previous x list = Some y; distinct (a#list
   done
 
 lemma allocate_alignUp:
-  "distinct list \<Longrightarrow>
-       x \<in> set list \<Longrightarrow>
-       (aligned_allocations spec (ptr :: machine_word) list) x =
-   Some (alignUp (the (allocate (ptr :: machine_word) spec list x))
-  (obj_bits_cdl (object_type (the (cdl_objects spec x))) (object_size_bits (the (cdl_objects spec x)))))"
+  "\<lbrakk> distinct list; x \<in> set list \<rbrakk> \<Longrightarrow>
+   aligned_allocations spec (ptr :: machine_word) list x =
+     Some (alignUp (the (allocate ptr spec list x))
+                   (obj_bits_cdl (object_type (the (cdl_objects spec x)))
+                                 (object_size_bits (the (cdl_objects spec x)))))"
   supply allocate.simps[simp]
   apply (induct list arbitrary: ptr; clarsimp)
   apply (clarsimp simp: aligned_allocations_def)
@@ -138,18 +140,21 @@ lemma allocate_alignUp:
   apply (subst in_right_map; clarsimp)
   done
 
-lemma some_previous: "\<lbrakk>a \<notin> set list; Some a = previous x (a#list)\<rbrakk> \<Longrightarrow> x = hd list"
+lemma some_previous:
+  "\<lbrakk>a \<notin> set list; Some a = previous x (a#list)\<rbrakk> \<Longrightarrow> x = hd list"
   apply (induct list arbitrary: x a; clarsimp)
   apply (metis Some_to_the empty_iff list.exhaust_sel list.set(1)
                not_in_previous option.distinct(1) previous.simps(3) set_ConsD)
   done
 
-lemma previous_cons[simp]: "a \<notin> set list \<Longrightarrow> p \<noteq> a \<Longrightarrow>
-     Some p = previous x (a # list) \<Longrightarrow> previous x (a # list) = previous x list"
+lemma previous_cons[simp]:
+  "\<lbrakk> a \<notin> set list; p \<noteq> a; Some p = previous x (a # list) \<rbrakk>
+   \<Longrightarrow> previous x (a # list) = previous x list"
   by (induct list; clarsimp)
 
-lemma allocate_previous: "\<lbrakk>distinct list; x \<in> set list; Some p = previous x list\<rbrakk> \<Longrightarrow>
-       (allocate ptr spec  list) x = Some (next_allocation spec (the (allocate ptr spec list p)) p)"
+lemma allocate_previous:
+  "\<lbrakk>distinct list; x \<in> set list; Some p = previous x list\<rbrakk> \<Longrightarrow>
+   (allocate ptr spec list) x = Some (next_allocation spec (the (allocate ptr spec list p)) p)"
   apply (subgoal_tac "p \<in> set list")
    supply allocate.simps[simp]
    apply (induct list arbitrary: p ptr)
@@ -178,50 +183,45 @@ lemma allocate_previous: "\<lbrakk>distinct list; x \<in> set list; Some p = pre
   done
 
 lemma aligned_allocate_previous:
-  "\<lbrakk>distinct list; x \<in> set list; Some p = previous x list \<rbrakk> \<Longrightarrow>
-    (aligned_allocations spec  ptr  list) x =
-       Some (alignUp ((next_allocation spec (the (allocate (ptr :: machine_word) spec list p)) p))
-         (obj_bits_cdl (object_type (the (cdl_objects spec x))) (object_size_bits (the (cdl_objects spec x)))))"
-  apply (unfold aligned_allocations_def mapp_def)
-  apply (subst arg_cong[OF allocate_previous,
-                        where f="map_option (\<lambda>ptr'. alignUp ptr' (spec_object_size spec x))"])
-     apply (fastforce)+
-  apply (metis option.simps(9) spec_object_size_def)
-  done
+  "\<lbrakk> distinct list; x \<in> set list; Some p = previous x list \<rbrakk> \<Longrightarrow>
+   aligned_allocations spec ptr list x =
+     Some (alignUp (next_allocation spec (the (allocate ptr spec list p)) p)
+                   (obj_bits_cdl (object_type (the (cdl_objects spec x)))
+                                 (object_size_bits (the (cdl_objects spec x)))))"
+  by (simp add: allocate_alignUp allocate_previous)
 
-abbreviation cptr_of ::
-  "(cdl_cptr \<times> bi_untyped_desc \<times> cdl_cap) option \<Rightarrow> cdl_cptr"
-  where
+abbreviation cptr_of :: "(cdl_cptr \<times> bi_untyped_desc \<times> cdl_cap) option \<Rightarrow> cdl_cptr" where
   "cptr_of \<equiv> \<lambda>x. fst (the x)"
 
-abbreviation cap_of ::
-  "(cdl_cptr \<times> bi_untyped_desc \<times> cdl_cap) option \<Rightarrow> cdl_cap"
-  where
+abbreviation cap_of :: "(cdl_cptr \<times> bi_untyped_desc \<times> cdl_cap) option \<Rightarrow> cdl_cap"  where
   "cap_of \<equiv> \<lambda>x. snd (snd (the x))"
 
-definition valid_derivations where
+definition valid_derivations ::
+  "cdl_state \<Rightarrow> (cdl_object_id \<times> cdl_object_id list) list \<Rightarrow>
+   (cdl_object_id \<Rightarrow> (cdl_cptr \<times> bi_untyped_desc \<times> cdl_cap) option) \<Rightarrow> bool"
+  where
   "valid_derivations spec untyped_derivations untyped_map \<equiv>
-    distinct (map fst untyped_derivations) \<and>
-    distinct_sets (map (set o snd) untyped_derivations) \<and>
-    (\<forall>family\<in>(set untyped_derivations).
-      let parent      = fst family;
-          parent_cap  = cap_of (untyped_map parent);
-          start       = Min (available_range (parent_cap));
-          children    = snd family
-      in
-        distinct children \<and>
-        (\<forall>child\<in>(set children).
-          let spec_child = the (cdl_objects spec child);
-              child_size = spec_object_size spec child
-          in
-            cdl_objects spec child \<noteq> None \<and>
-            object_type spec_child \<noteq> UntypedType \<and>
-            object_size_bits spec_child < 2 ^ word_bits \<and>
-            start \<le> start + 2 ^ child_size \<and>
-            child_size < word_size \<and>
-            is_aligned start child_size \<and>
-            start \<le> the (aligned_allocations spec start children child) + 2 ^ child_size \<and>
-            (previous child children \<noteq> None \<longrightarrow> start < the (allocate start spec children child)) \<and>
-            the (allocate start spec children child) \<in> available_range (parent_cap)))"
+     distinct (map fst untyped_derivations) \<and>
+     distinct_sets (map (set o snd) untyped_derivations) \<and>
+     (\<forall>family\<in>(set untyped_derivations).
+       let parent      = fst family;
+           parent_cap  = cap_of (untyped_map parent);
+           start       = Min (available_range (parent_cap));
+           children    = snd family
+       in
+         distinct children \<and>
+         (\<forall>child\<in>(set children).
+           let spec_child = the (cdl_objects spec child);
+               child_size = spec_object_size spec child
+           in
+             cdl_objects spec child \<noteq> None \<and>
+             object_type spec_child \<noteq> UntypedType \<and>
+             object_size_bits spec_child < 2 ^ word_bits \<and>
+             start \<le> start + 2 ^ child_size \<and>
+             child_size < word_size \<and>
+             is_aligned start child_size \<and>
+             start \<le> the (aligned_allocations spec start children child) + 2 ^ child_size \<and>
+             (previous child children \<noteq> None \<longrightarrow> start < the (allocate start spec children child)) \<and>
+             the (allocate start spec children child) \<in> available_range (parent_cap)))"
 
 end
